concurrency/disciplined/sharedexclusive-linearatomic/CircularRange.i.dfy
@@ -1,0 +1,153 @@
+include "../../../lib/Lang/NativeTypes.s.dfy"
+include "../common/Limits.i.dfy"
+
+module CircularRange {
+  import opened NativeTypes
+  import opened Limits
+
+  type Index = i: int | 0 <= i < FixedSize()
+
+  function NextIndex(i: Index): Index
+  {
+    if i == FixedSize() - 1 then 0 else i + 1
+  }
+
+  function PrevIndex(i: Index): Index
+  {
+    if i == 0 then FixedSize() - 1 else i - 1
+  }
+
+  datatype Range = 
+    | Everything
+    | Partial(start: Index, end: Index)
+  {
+    predicate HasNone()
+    {
+      Partial? && start == end
+    }
+
+    predicate HasSome()
+    {
+      !HasNone()
+    }
+
+    predicate Contains(i: Index)
+    {
+      match this {
+        case Everything => true
+        case Partial(start, end) =>
+          if start <= end then
+            (start <= i < end)
+          else
+            (start <= i || i < end)
+      }
+    }
+
+    predicate OverlapsWith(other: Range)
+    {
+      exists i : Index ::
+        (Contains(i) && other.Contains(i))
+    }
+
+    predicate DisjointsWith(other: Range)
+    {
+      !OverlapsWith(other)
+    }
+
+    predicate IsSuperOf(other: Range)
+    {
+      forall i : Index ::
+        (other.Contains(i) ==> Contains(i))
+    }
+
+    predicate IsSubOf(other: Range)
+    {
+      forall i : Index ::
+        (Contains(i) ==> other.Contains(i))
+    }
+
+    function GetComplement(): Range
+    {
+      match this {
+        case Everything => Partial(0, 0)
+        case Partial(start, end) =>
+          if start == end then 
+            Everything
+          else
+            Partial(end, start)
+      }
+    }
+
+    lemma ComplementCorrect(range: Range)
+      ensures
+        var range' := range.GetComplement();
+        && range.DisjointsWith(range')
+        && forall i : Index ::
+          (range.Contains(i) || range'.Contains(i))
+    {
+    }
+
+  }
+
+
+  // lemma DisjointRangesValidBetween(a: Range, b: Range)
+  //   requires !OverlapsWith(a, b)
+  //   requires !a.Nothing? && !b.Nothing?
+  //   ensures a.Partial? && b.Partial?
+  // {
+  //   if a.Everything? {
+  //     if b.Partial? {
+  //       assert Contains(a, b.start);
+  //     } else {
+  //       assert Contains(a, 0);
+  //       assert Contains(b, 0);
+  //     }
+  //     assert false;
+  //   }
+    
+  //   if b.Everything? {
+  //     if a.Partial? {
+  //       assert Contains(b, a.start);
+  //     } else {
+  //       assert Contains(a, 0);
+  //       assert Contains(b, 0);
+  //     }
+  //     assert false;
+  //   }
+
+  //   assert a.Partial? && b.Partial?;
+  // }
+
+  // function GetBetween(a: Range, b: Range): Range
+  //   requires !OverlapsWith(a, b)
+  // {
+  //   if a.Nothing? || b.Nothing? then
+  //     Nothing
+  //   else (
+  //     DisjointRangesValidBetween(a, b);
+  //     if a.end == b.start then Nothing
+  //     else Partial(a.end, b.start)
+  //   )
+  // }
+
+  // // if i is not in range, then i is in the copmlement (vice versa)
+  // lemma RangeComplement(i: Index, range: Range)
+  //   ensures !Contains(range, i) == Contains(GetComplement(range), i);
+  // { 
+  // }
+
+  // lemma RangeInclusion(a: Index, b: Index, c: Index)
+  //   requires a != b && a != c
+  //   requires Contains(Partial(a, b), c)
+  //   ensures Contains(Partial(c, a), b);
+  // {
+  // }
+
+  // // lemma RangeNext(start: Index, end: Index, i: Index)
+  // //   requires start != end
+  // //   requires start != NextIndex(end)
+  // //   requires Contains(Partial(start, NextIndex(end)), i);
+  // // {
+  // //   assert Contains(Partial(start, end), i) || end == i;
+  // // }
+}
